theories/run_prop_hard.v
@@ -5,27 +5,6 @@ From det Require Import zify_ssreflect.
 Section s.
   Variable u : Unif.
 
-  (* Lemma next_alt_exp_same {s A r}:
-    expand u s A = r -> is_fail r = false -> is_solved r = false ->
-      next_alt false A = Some A.
-  Proof.
-    move=> <-; elim: A s {r} => //=.
-    - move=> A HA s B HB s1.
-      case: ifP => dA.
-        have:= HB s; case: expand => //=s' B'/(_ erefl)->//.
-      have:= HA s1; case: expand => //= _ _ /(_ erefl)->//.
-    - move=> A HA B0 _ B HB s; case: ifP => dA.
-        rewrite is_dead_expand//.
-      have:= HA s; case X: expand => //=[s' A'|s' A'|s' A'] /(_ erefl).
-        move=> /(_ erefl)->; rewrite (expand_not_failed _ X notF) (expand_not_solved_not_success _ X notF)//.
-        move=> /(_ erefl)->; rewrite (expand_not_failed _ X notF) (expand_not_solved_not_success _ X notF)//.
-      have [[??]sA] := expand_solved_same _ X; subst.
-      rewrite sA success_failed//.
-      have:= HB (get_substS s A').
-      case Y: expand => //=[s'' B'|s'' B'] /(_ erefl erefl) ->//.
-  Qed. *)
-
-
   Lemma runb_success1 {A} s: 
     success A -> runb u s A (Some (get_substS s A)) (build_na A (next_alt true A)) 0.
   Proof.
@@ -358,20 +337,6 @@ Section s.
         else dead1 X
       else X
     else if is_dead A' then dead1 X else cutr X.
-
-  (* Lemma build_or_state_inj {cn A A1} A2:
-    build_or_state cn A A1 ->
-      build_or_state cn A A2 -> A1 = A2.
-  Proof.
-    rewrite/build_or_state.
-    case: eqP => [?|???]; subst => //.
-    case: r => [???|]; subst => //.
-    case: next_alt => [?|??]; subst => //.
-    (* TODO: solve this issue by removing the existential and
-       add the state in option None in runb *)
-    move=> [A1 [dA1 ?]] [A2 [dA2 ?]]; subst.
-    repeat f_equal.
-  Admitted. *)
 
   Lemma runb_none_dead_res {s A B cn} :
     runb u s A None B cn -> dead1 B = B.
@@ -770,89 +735,6 @@ Section s.
         by rewrite next_alt_cutr if_same.
   Qed.
 
-
-  (* Section kill_top.
-    Fixpoint kill_top A :=
-      match A with
-      | OK | CallS _ _ | CutS | Bot | Dead => A
-      | Or A s B => if is_dead A then (Or A s (kill_top B)) else (Or (kill_top A) s B)
-      | And A B0 B =>
-          let A' := kill_top A in
-          if success A' then And A' B0 (kill_top B)
-          else And A' B0 B
-      end.
-
-    Fixpoint is_kill_top A :=
-      match A with
-      | Top => true
-      | OK | CallS _ _ | CutS | Bot | Dead => false
-      | Or A s B => if is_dead A then is_kill_top B else is_kill_top A
-      | And A B0 B =>
-        if success A then is_kill_top B
-        else is_kill_top A
-      end.
-
-    Lemma is_dead_kill_top {A}: is_dead (kill_top A) = is_dead A.
-    Proof.
-      elim: A => //=.
-      - by move=> A HA s B HB; rewrite fun_if /= HB HA if_same.
-      - by move=> A HA B0 _ B HB; rewrite fun_if/= HA if_same.
-    Qed.
-
-    Lemma success_kill_top {A}: success A -> (kill_top A) = A.
-    Proof.
-      elim: A => //=.
-      - move=> A HA s B HB; case: ifP => [dA sB|dA sA]/=; rewrite ?is_dead_kill_top//?dA ?HB//HA//.
-      - move=> A HA B0 _ B HB /andP[sA sB]/=; rewrite HA//HB//if_same//.
-    Qed.
-
-    Lemma is_kill_top_kill_top {A}:
-      is_kill_top (kill_top A) = false.
-    Proof.
-      elim: A => //=.
-      - move=> A HA s B HB; by case: ifP => dA/=; rewrite?is_dead_kill_top dA//.
-      - move=> A HA B0 _ B HB; case: ifP => sA/=; rewrite sA//.
-    Qed.
-
-    Lemma is_kill_top_exp {s1 A r}: is_kill_top A -> expand u s1 A = r -> is_expanded r.
-    Proof.
-      move=> +<-{r}.
-      elim: A s1 => //=.
-      - move=> A HA s B HB s1; case: ifP => dA k/=.
-          have:= HB s k; case X: expand => //.
-        have:= HA s1 k; case: expand => //.
-      - move=> A HA B0 _ B HB s1.
-        case: ifP => s k.
-          rewrite succes_is_solved//.
-          have:= HB (get_substS s1 A) k; case: expand => //.
-        have:= HA s1 k; case: expand => //.
-    Qed.
-
-    Lemma is_kill_topF_kill_top_refl {A}: is_kill_top A = false -> kill_top A = A.
-    Proof.
-      elim: A => //=.
-      - move=> A HA s B HB; case: ifP => dA k; rewrite?HA//?HB//.
-      - move=> A HA B0 _ B HB; case: ifP => sA k.
-          by rewrite HB// success_kill_top// if_same.
-        by rewrite HA// sA.
-    Qed.
-
-    Lemma get_substS_kill_top {s A}: get_substS s (kill_top A) = get_substS s A.
-    Proof.
-      elim: A s => //=.
-      - by move=> A HA s B HB s1; case: ifP => dA/=; rewrite?is_dead_kill_top dA//.
-      - move=> A HA B0 _ B HB s; rewrite 2!fun_if/= HA HB if_same.
-        case:ifP => //sA.
-          rewrite success_kill_top// sA//.
-        case: ifP => // skA.
-        (* THIS IS WRONG! *)
-    Abort.
-
-    Lemma dead_kill_top {A}: dead1 (kill_top A) = dead1 A.
-    Proof. elim: A => //=[A HA s B HB|A HA B0 _ B HB]; rewrite fun_if/= HA HB if_same//. Qed.
-
-  End kill_top. *)
-
   Lemma run_and_correct_successL {s0 sn A B0 B A' B0' B' b}:
     success A -> next_alt true A = None ->
     runb u s0 (And A B0 B) sn (And A' B0' B') b ->
@@ -880,7 +762,6 @@ Section s.
       case eA1: expand => //[B1'][?]; subst.
       have {IH} := IH _ _ _ erefl _ _ _ erefl.
       rewrite next_alt_cutl success_cut => /(_ sA1 erefl).
-      (* have ? := expand_cb_same_subst _ eA1; subst. *)
       rewrite ges_subst_cutl// cutl2 if_same dead_cutl.
       move=> [rB1'[??]]; subst.
       rewrite cutr2 dead_cutr !if_same.
@@ -906,56 +787,6 @@ Section s.
       rewrite is_dead_dead; repeat split.
       apply: run_dead fB1 X.
   Qed.
-
-  (* Lemma runb_kill_top {s A s2 r n}: runb u s (kill_top A) s2 r n -> runb u s A s2 r n.
-  Proof.
-    elim: A s s2 r n => //=.
-    - move=> s1 s2 r n H; apply: run_step H => //.
-    - move=> A HA s B HB s1 s2 r n.
-      case: ifP => dA /[dup]/runb_or0->{n}/[dup]/runb_same_structure/=; case: r => //= A' _ B' /eqP<- H.
-        have [b[{}H ?]] := run_ko_left1 (is_dead_is_ko dA) H; subst.
-        have {HA}HB := HB _ _ _ _ H.
-        apply: run_ko_left2 (is_dead_is_ko dA) HB.
-      have [n1] := run_or_complete H.
-      case: s2 H => [s2|] H.
-        move=> [].
-          move=> [H1?]; subst.
-          have {}HA := HA _ _ _ _ H1.
-          by have:= run_or_correct_left HA s B.
-        rewrite /get_dead is_dead_kill_top dA.
-        move=> [kA' [H1 H2]].
-        have {H H1 HB}HA := HA _ _ _ _ H1.
-        have := run_or_correct_left HA.
-        move=> /(_ _ _ _ _ _ H2).
-        rewrite dA//.
-      move=> [] /HA{}HA.
-      case:eqP => Hn1; subst.
-        move=> [[n2 rB] [dA' dB']].
-        have := run_or_correct_left HA.
-        move=>/(_ _ _ _ _ _ rB).
-        rewrite dA//.
-      move=> [?[dA' Hr]]; subst.
-      have:= run_or_correct_left HA.
-      case: eqP => //.
-    - move=> A HA B0 HB0 B HB s r C n.
-      case:ifP => skA H; have:= runb_same_structure _ H; case: C H => //= A' B0' B' H _.
-        have rkA := runb_success1 s skA.
-        case X: next_alt => [A''|]/=; last first.
-          have {H} := run_and_correct_successL skA X H.
-          move=> [rkB [??]]; subst.
-          have {rkB} HB := HB _ _ _ _ rkB.
-          have {}HA := HA _ _ _ _ rkA.
-          rewrite dead_kill_top.
-          move: HA HB rkA.
-          rewrite X/=dead_kill_top.
-          set s' := get_substS _ _ => HA HB rkA.
-
-          admit.
-        admit.
-      admit.
-  Admitted. *)
-
-
 
   (*Lemma run_and_correct {s0 sn A B0 B A' B0' B' b}:
     runb u s0 (And A B0 B) sn (And A' B0' B') b ->
